# 2.6

## Follow Up
This exercise asks me to implement one and two as a pair implemented by lambda expressions, the text uses these two definitions:

``` racket
(define zero (lambda (f) (lambda (x) x))) Procedure that applies x 0 times

(define (add-1 n)
  (lambda (f) (lambda (x) (f ((n f) x))))) 
```

for implementing 0 and add-1

## Following the Suggestions
The text suggests to use the substituion model to evaluate (add-1 zero) and to give a direct definition of the addition procedure:

``` racket
(add-1 zero)
-> (lambda (f) (lambda (x) (f ((zero f) x)))) 
-> (lambda (f) (lambda (x)
                (f
                    (
                    ((lambda (f) (lambda (x) x)) f)
                        x)
                )))
-> (lambda (f) (lambda (x)
                (f
                    (
                    ((lambda (f) (lambda (x) x)) f)
                        x)
                )))
```

f->x->x; f = f  
f->x->x; x = x  
f->x->x->x "adds one more application to zero"

So, time for the second hint, how I would define an addition between numbers represented by procedures?

an addition between two data is a combination between two datas:
(add p1 p2)

if p1 = f->x->x = 0  
and p2 = f->x->x->x = 1

then (add p1 p2) should return f->x->x->x
## Implementing add in the Church's way
### First attempt
``` racket
(define (add-p n1 n2) 
    (lambda (f) 
        (lambda (x) (f (((n1 f) n2 ) x)))))
```

If I call add-p with zero and zero, the procedure should return 0?

TEST:

substitution model:

``` racket
(add-p zero zero)
->(lambda (f)
    (lambda (x)
        (f 
                (((lambda (f)
                        (lambda (x) x)) f)
                         (lambda (f) 
                            (lambda (x) x))) x))))
```


NEGATIVE.

### Second attempt
I have to retrace the add-1 procedure, also I guess that the addition procedure is a composition:
((lambda (f) (lambda (x) x) f)->(lambda (x) x)  
((lambda (x) x) x) -> x  
(lambda (f) (lambda (x) (f x))) = 1  
(lambda (f) (lambda (x) (f (f x)))) = 2  

``` racket
(define (add n1 n2) (lambda (f)
        (lambda (x) (f ((n2 (n1 f)) x)))
    )
)
```
``` racket
(add zero zero)
-> (lambda (f) 
        (lambda (x) (f ((zero (zero f)) x)))
    )
-> (lambda (f)
        (lambda (x) 
            (f (((lambda (f) (lambda (x) x)) 
                ((lambda (f) (lambda (x) x)) f)) 
                    x)))
    )

((lambda (f) (lambda (x) x)) f) -> (lambda (x) x)
((lambda (f) (lambda (x) x)) ((lambda (x) x))-> (lambda (x) x)
((lambda (x) x) x)-> x
(lambda (f) (lambda (x) (f x)))
```
INCORRECT

### Third attempt
RETRY:
``` racket
(define (add n1 n2) (lambda (f)
        (lambda (x) ((n1 ((n2 f) x)) f)
    )
)
```


((lambda (f) (lambda (x) x) f) = (lambda (x) x)  
((lambda (x) x) x) = x  
((lambda (f) (lambda (x) x)) x) = (lambda (x) x)  
((lambda (x) x) f) = x  
(lambda (f) (lambda (x) x)) vvv  


add-1 procedure
``` racket
(define (add-1 n)
  (lambda (f) (lambda (x) (f ((n f) x))))) 
```
``` racket
(add-1 one)
-> (lambda (f) (lambda (x) (f ((one f) x))))
-> (lambda (f) 
        (lambda (x) (f (((lambda (f) (lambda (x) (f x))) f) x)))
    )
-> ((lambda (f) (lambda (x) (f x))) f) -> (lambda (x) (f x))
    ((lambda (x) (f x)) x) -> (f x)
```

### Fourth Attempt
RETRY:
``` racket
(define (add n1 n2) (lambda (f)
        (lambda (x) ((n1 f) ((n2 f) x)))
    )
)
```

``` racket
(add zero one)
-> (lambda (f) (lambda (x) ((zero f) ((one f) x))))
-> (lambda (f) (lambda (x) 
        (((lambda (f) (lambda (x) x)) f) ((lambda (f) (lambda (x) (f x))) x)))    
    )
-> ((lambda (f) (lambda (x) (f x))) f) = (lambda (x) (f x))
-> ((lambda (x) (f x)) x) = (f x)
    ((lambda (x) x) (f x)) = (f x)
```

    VVV