An illustrative exercise which asks me to perform the substitution model for normal order to the GCD procedure reported below:

(define (gcd a b)
  (if (= b 0)
      a
      (gcd b (remainder a b))))

with input a = 206; b = 40.


Let's try it:

(gcd 206 40)  
(gcd 40 (remainder 206 40))  
(if (= (remainder 206 40) 0) 40 (gcd (remainder 206 40) (remainder 40 (remainder 206 40))))  
false
(if (= (remainder 40 (remainder 206 40)) 0)  
	(remainder 206 40)  
	(gcd (remainder 40 (remainder 206 40)) (remainder (remainder 206 40) (remainder 40 (remainder 206 40)))))  
false  
(if (= (remainder (remainder 206 40) (remainder 40 (remainder 206 40))) 0)  
	(remainder 40 (remainder 206 40))  
	(gcd (remainder (remainder 206 40) (remainder 40 (remainder 206 40))) (remainder (remainder 40 (remainder 206 40)) (remainder (remainder 206 40) (remainder 40 (remainder 206 40)))))  
	false  
	(if (= (remainder (remainder 40 (remainder 206 40)) (remainder (remainder 206 40) (remainder 40 (remainder 206 40)))) 0)  
		(remainder (remainder 206 40) (remainder 40 (remainder 206 40)))  
		true  
		
remainder op = 18

		
(gcd 206 40)  
(gcd 40 6) 1  
(gcd 6 4) 2  
(gcd 4 2) 3  
(gcd 2 0) 4  
2  

APPLICATIVE ORDER = 4
